Checkpoint progress towards removing fs_invariant, since it will not be true in the presence of renames.  Instead rely on pathname unique for tmpdir. This changes specs and proofs but appears to be simpler. The tricky one is the proof of [path_eval_addlink'], which is sketched out in this commit.

src/FS/MailServerAPI.v
@@ -57,7 +57,6 @@ Inductive mailfs_step_allowed : forall T, fsOpT T -> nat -> Prop :=
 *)
 
 Definition invariant (fs : FS) :=
-  fs_invariant fs /\
   unique_pathname fs tmpdir.
 
 Definition mailfs_step T (op : fsOpT T) tid s r s' :=
@@ -112,12 +111,10 @@ Proof.
   unfold invariant, unique_pathname; intuition; repeat deex.
   - rewrite <- H in *.
     eauto.
-  - rewrite H in H0; eexists; intuition eauto.
-    eapply H2. rewrite H. eauto.
-  - rewrite H in *.
-    eauto.
-  - rewrite <- H in H0; eexists; intuition eauto.
-    eapply H2. rewrite <- H. eauto.
+  - specialize (H0 node node').
+    rewrite H in H1.
+    rewrite H in H2.
+    specialize (H0 H1 H2); auto.
 Qed.
 
 Lemma path_eval_root_create: forall fs pn dirnum h name,
@@ -130,69 +127,173 @@ Proof.
   eapply path_eval_root_addlink in H0; eauto.
 Qed.
 
-Lemma path_eval_root_create': forall fs pn dirnum h name node',
+Lemma valid_link_addlink_does_not_exists: forall fs dirnum name h node' node'' startdir name0,
     name <> "." ->
     name <> ".." ->
-    fs_invariant fs ->
     does_not_exist fs dirnum name ->
-    file_handle_unused fs h ->
-    file_handle_valid fs h ->
-    path_eval_root fs pn (DirNode dirnum) ->
-    path_eval_root (create_file dirnum h name fs) pn node' ->
-    node' = (DirNode dirnum).
+    valid_link fs startdir name0 node'' ->
+    valid_link (add_link dirnum (FileNode h) name fs) startdir name0 node' ->
+    valid_link fs startdir name0 node'.
 Proof.
   intros.
-  eapply path_eval_root_addlink' in H6 as H6x; eauto.
-  eapply path_eval_root_updfile' in H6x.
-  eapply path_eval_root_eq; eauto.
-
-  unfold fs_invariant, unique_dirents; intros.
-  apply valid_link_updfile' in H7.
-  apply valid_link_updfile' in H8.
-  eapply H1; eauto.
-  eapply path_eval_root_updfile; eauto.
+  inversion H3; subst.
+  apply Graph.add_spec in H4.
+  intuition; subst. 
+  inversion H5; subst. clear H5.
+  destruct H1.
+  eexists.
+  inversion H2; subst; eauto; try congruence.
+  apply ValidDot.
+  eapply ValidDotDot.
+  apply Graph.add_spec in H4.
+  intuition; subst; try congruence.
+  eauto.
+  eapply ValidDotDotRoot.
+  unfold add_link; simpl; auto.
 Qed.
 
-Lemma invariant_create : forall dirnum h name fs,
+Lemma path_eval_addlink' : forall fs dirpn startdir dirnum h name node,
+    name <> "." ->
+    name <> ".." ->
+     (forall node node' : Node,
+       path_evaluates fs (DirNode startdir) dirpn node ->
+       path_evaluates fs (DirNode startdir) dirpn node' -> node' = node) ->
+    does_not_exist fs dirnum name ->
+    path_evaluates fs (DirNode startdir) dirpn (DirNode dirnum) ->
+    path_evaluates (add_link dirnum (FileNode h) name fs) (DirNode startdir) dirpn node ->
+    DirNode dirnum = node.
+Proof.
+  intros.
+  generalize dependent fs; intros.
+  induction H3.
+  + inversion H4; subst; auto.
+  + inversion H4; subst; clear H4.
+    eapply valid_link_addlink_does_not_exists in H8; eauto.
+    inversion H11; subst.
+    eapply valid_link_addlink_does_not_exists in H9; eauto.
+    inversion H12; subst; clear H12.
+    eapply valid_link_addlink_does_not_exists in H9; eauto.
+    exfalso. admit.
+  + inversion H4; subst; clear H4.
+    eapply valid_link_addlink_does_not_exists in H11; eauto.
+    {
+      eapply valid_link_addlink_does_not_exists in H10; eauto.
+      assert (inum = inum0).
+      admit.
+      subst.
+      apply IHpath_evaluates; try eassumption.
+      admit.
+    }
+    { 
+      eapply valid_link_addlink_does_not_exists in H10; eauto.
+      admit.  (* H10 and H3 and H1 *)
+    }
+  + inversion H4; subst. clear H4.
+    eapply valid_link_addlink_does_not_exists in H10; eauto.
+    {
+      eapply valid_link_addlink_does_not_exists in H9; eauto.
+      admit.  (* H9 and H3 and H1 *)
+    }
+    eapply valid_link_addlink_does_not_exists in H9; eauto.
+    assert (sympath0 = sympath).
+    admit.
+    subst.
+    assert (symtarget = node).
+    subst.
+    eapply IHpath_evaluates1.
+    admit.
+    auto.
+    assert (node = symtarget0).
+    admit.
+    subst.
+    auto.
+    apply IHpath_evaluates2; auto.
+    admit.
+    assert (symtarget0 = symtarget).
+    admit.
+    subst.
+    auto.
+ Admitted.
+
+Lemma path_eval_root_addlink' : forall fs dirnum name dirpn h node,
     name <> "." ->
     name <> ".." ->
     does_not_exist fs dirnum name ->
-    file_handle_unused fs h ->
-    file_handle_valid fs h ->
-    path_eval_root fs tmpdir (DirNode dirnum) ->
-    invariant fs ->
-    invariant (create_file dirnum h name fs).
+    unique_pathname fs dirpn ->
+    path_eval_root fs dirpn (DirNode dirnum) ->
+    path_eval_root (add_link dirnum (FileNode h) name fs) dirpn node ->
+    DirNode dirnum = node.
 Proof.
-  unfold invariant; intuition idtac.
-  eapply fs_invariant_create; eauto.
-  unfold unique_pathname in *; repeat deex.
-  exists (DirNode dirnum); split.
-  eapply path_eval_root_create in H4; eauto.
+  unfold unique_pathname, path_eval_root.
   intros.
-  eapply path_eval_root_create'; eauto.
+  eapply path_eval_addlink'; try eassumption.
+Qed.
+
+Lemma path_eval_root_create': forall fs pn node dirnum h name,
+    name <> "." ->
+    name <> ".." ->
+    does_not_exist fs dirnum name ->
+    unique_pathname fs pn ->
+    path_eval_root fs pn (DirNode dirnum) ->
+    path_eval_root (create_file dirnum h name fs) pn node ->
+    DirNode dirnum = node.
+Proof.
+  intros.
+  unfold create_file in *.
+  eapply path_eval_root_updfile with (h := h) (data := "") in H3.
+  eapply path_eval_root_addlink' with (fs := (upd_file h "" fs)); try eassumption.
+  unfold upd_file; simpl.
+  admit.
+Admitted.
+
+Lemma path_unique_eq: forall fs dirnum pn node',
+    unique_pathname fs pn ->
+    path_eval_root fs pn (DirNode dirnum) ->
+    path_eval_root fs pn node' ->
+    node' = DirNode dirnum.
+Proof.
+  intros.
+  unfold unique_pathname in *.
+  specialize (H (DirNode dirnum) node').
+  specialize (H H0 H1).
+  auto.
 Qed.
 
 Lemma path_unique_create_inum_eq: forall fs pn dirnum dirnum0 h name,
-    invariant fs ->
+    unique_pathname fs pn ->
     does_not_exist fs dirnum0 name ->
     file_handle_unused fs h ->
     file_handle_valid fs h ->
-    invariant (create_file dirnum0 h name fs) ->
+    unique_pathname (create_file dirnum0 h name fs) pn ->
     path_eval_root fs pn (DirNode dirnum0) ->
     path_eval_root (create_file dirnum0 h name fs) pn (DirNode dirnum) ->
     dirnum = dirnum0.
 Proof.
   intros.
   assert (DirNode dirnum = DirNode dirnum0) as Hinum.
-  destruct H; intuition idtac.
-  eapply path_eval_root_updfile in H4 as Hx.
-  eapply path_eval_root_addlink in Hx.
-  2: apply does_not_exist_updfile'; eauto.
-  eapply path_eval_root_eq.
-  3: apply Hx.
-  2: eauto.
-  unfold invariant in *; intuition idtac.
+  eapply path_eval_root_create in H4 as Hx; try eassumption.
+  eapply path_unique_eq in H3; try eassumption.
   inversion Hinum; auto.
+Qed.
+
+Lemma invariant_create : forall fs pn dirnum h name,
+    name <> "." ->
+    name <> ".." ->
+    unique_pathname fs pn ->
+    does_not_exist fs dirnum name ->
+    file_handle_unused fs h ->
+    file_handle_valid fs h ->
+    path_eval_root fs pn (DirNode dirnum) ->
+    unique_pathname (create_file dirnum h name fs) pn.
+Proof.
+  intros.
+  unfold unique_pathname.
+  intros.
+  assert (DirNode dirnum = node).
+  eapply path_eval_root_create' in H6; try eassumption.
+  subst.
+  symmetry.
+  eapply path_eval_root_create' in H7; try eassumption.
 Qed.
 
 Lemma create_file_comm: forall fs dirnum h0 h1 name1 name0,
@@ -242,8 +343,8 @@ Proof.
       2: reflexivity; eauto.
       econstructor; eauto.
       eauto.
-      eapply invariant_create; eauto.
 
+      apply invariant_create; try eauto.
       (* some come from econstructor; others form invariant_create *)
       Unshelve.
       all: auto.
@@ -259,8 +360,7 @@ Proof.
       all: try unfold create_file; eauto.
 
       apply create_file_comm; auto.
-      eapply invariant_create; eauto.
-
+      apply invariant_create; try eauto.
       Unshelve.
       all: auto.
 
